\section{Deciding Temporal Logic Queries}

\begin{frame}[plain]
  \setbeamercolor{background canvas}{bg=oceangreen!15}
  \vskip11ex
  \begin{center}
    \Huge
    \color{oceangreen}\bfseries \insertsection
  \end{center}
\end{frame}

\begin{frame}{Deciding Temporal Logic Queries}
  Query:
  \[ \AG \qst_1 \{p,q\} \]
  
  Naive approach:
  \begin{itemize}
    \item fixed set of $k$ atomic propositions
    \item take all $2^{2^k}$ propositional formulas
    \item substitute the placeholder
    \item verify each resulting formula
    \item return set of maximally strong solutions
  \end{itemize}
\end{frame}


\begin{frame}{Example Kripke Structure}
  \begin{center}
    \begin{tikzpicture}[->,>=stealth',shorten >=1pt,auto,
        node distance=12em,thick]
    \tikzstyle{every state}=[fill=oceangreen!19,minimum width=5em,align=center,inner sep=4pt]
    \tikzstyle{every pin}=[distance=2ex]
    \tikzstyle{every pin edge}=[-,draw=none,thin]

      \node[initial,state,pin=above :{$s_0$}] (s0) {$p$\\$\lnot q$\\$r$};
      \node[state,pin=right :{$s_2$}]         (s2) [below right of=s0] {$p$\\$q$\\$r$};
      \node[state,pin=above :{$s_1$}]         (s1) [above right of=s2] {$\lnot p$\\$q$\\$r$};
      

      \path (s0) edge (s1)
            (s0) edge [bend left] (s2)
            (s1) edge [loop right] ()
            (s2) edge [bend left] (s0)
                 edge (s1);
    \end{tikzpicture}
  \end{center}
\end{frame}

\subsection[One Placeholder]{Queries with One Placeholder}

%\begin{frame}{Basics}
%  Propositional formulas $\PF(P)$
%  \[ \PF(\{p\}) = \{ \true, \false, p, \lnot p\} \]
%  
%  $\mcJ(\mcL)$ set of all join-irreducible elements of \
%  
%  $\chi$CTL(\mcL) formula for $\qst_1\{p\}$:
%  \[ (p \land \uparrow\{p\}) \lor (\lnot p \land \uparrow\{\lnot p\}) \]
%\end{frame}


\begin{frame}{Simple Query $\qst_1\{p\}$}
  Propositional formulas:
  \[ \PF(\{p\}) = \{ \true, \false, p, \lnot p\} \]
  
  Formula $p$ holds in $s_0$
  
  Solution is $\uparrow\{p\}$
  
  
\end{frame}

\begin{frame}{Simple Query $\qst_1\{p\}$}
  Arbitrary state $s$:
  \[ \llbracket \qst_1\{p\} \rrbracket (s) = \begin{cases}
       \uparrow\{p\} & \text{if } \llbracket p \rrbracket (s) = \true \\
       \uparrow\{\lnot p\} & \text{if } \llbracket \lnot p \rrbracket (s) = \true \\
     \end{cases} 
  \]
  
  $\chi$CTL(\mcL) formula for $\qst_1\{p\}$:
  \[ (p \land \uparrow\{p\}) \lor (\lnot p \land \uparrow\{\lnot p\}) \]
\end{frame}

\begin{frame}{Query $\qst_1$}
  Solution to the query $\qst_1$ for an arbitrary set of propositions:
  \[ \llbracket \qst_1 \rrbracket (s) = \uparrow\{j\} \text{ iff } \llbracket j \rrbracket (s) = \true
  \]
  
  Where $j\in\mcJ(\PF(\qst_1))$
\end{frame}

\begin{frame}{Syntactic Translation $\T_\uparrow$}
  Translation into $\chi$CTL(\mcL) formula over the lattice $\U(\PF(\qst_1))$:
  \[ 
    \T_\uparrow(\qst_1) \triangleq \bigvee_{j\in\mcJ(\PF(\qst_1))} (j \land \uparrow j)
  \]
\end{frame}

\begin{frame}{Generalized Translation $\T_f$}
  Replace $\uparrow$ by a function $f : \mcJ(\PF(\qst_1)) \to \mcL$

  Generalized translation function:
  \[ 
    \T_f(\qst_1) \triangleq \bigvee_{j\in\mcJ(\PF(\qst_1))} (j \land f(j))
  \]
\end{frame}

\begin{frame}{Extending Translation $\T_f$}
  Extend $\T_f$ from $\qst_1$ to all logic queries:
  \[ 
    \T_f(\phi[\qst_1]) \triangleq \phi[\T_f(\qst_1)]
  \]
  
  \begin{example}[Solution for $\EX \qst_1\{p,q\}$]
    Apply transformation:
    \[ \T_f(\EX \qst_1\{p,q\}) = \EX\T_f( \qst_1\{p,q\}) \]
  \end{example}
\end{frame}

\begin{frame}{Solution for $\EX \qst_1\{p,q\}$}
  \begin{example}[Expand $\T_f( \qst_1\{p,q\})$]
    \begin{align*}
      \T_f( \qst_1\{p,q\}) 
        =   &(p \land q \land \uparrow\{p\land q\}) \\
        \lor&(p \land \lnot q \land \uparrow\{p\land \lnot q\}) \\
        \lor&(\lnot p \land q \land \uparrow\{\lnot p\land q\}) \\
        \lor&(\lnot p \land \lnot q \land \uparrow\{\lnot p\land \lnot q\})
    \end{align*}
  \end{example}
\end{frame}

\begin{frame}{Solution for $\EX \qst_1\{p,q\}$}
  \begin{example}[Evaluate resulting formula]
    \begin{align*}
      & \llbracket \EX \T_f( \qst_1\{p,q\}) \rrbracket (s_0) \\
        =& \llbracket \EX \T_f( \qst_1\{p,q\}) \rrbracket (s_1) \lor \llbracket \EX \T_f( \qst_1\{p,q\}) \rrbracket (s_2) \\
        =& \uparrow\{\lnot p\land q\} \lor \uparrow\{p\land q\} \\
        =& \uparrow\{p\land q, \lnot p\land q\} 
    \end{align*}
  \end{example}
\end{frame}

\subsection{Multiple Placeholders}%%%%%%%%%%%%%%%%%%%%%%%%%%%%%%%%%%%%%%%%

\begin{frame}{Decide Queries with Multiple Placeholders}
  Queries with multiple placeholders $\phi[\qst_1,\ldots,\qst_n]$:
  \begin{itemize}
    \item set of all solutions $L = \PF(\qst_1)\times \cdots \times \PF(\qst_n)$
  \end{itemize}
\end{frame}

\frame{\Huge Hier fehlt mir die Idee wie ich Multiple Placeholders verständlich erklären kann}



\subsection{Negative Queries}%%%%%%%%%%%%%%%%%%%%%%%%%%%%%%%%%%%%%%%%

\begin{frame}{Decide Negative Queries}
  Negative queries $\phi[\qst_1]$:
  \begin{itemize}
    \item transform negative query into positive one
    \item apply query checking
    \item postprocess result
  \end{itemize}
\end{frame}

\begin{frame}{Transform into Positive Query}
  Transform negative query $\phi[\qst_1]$ into positive query denoted by $\myN$
  \begin{itemize}
    \item remove all negations in front of $\qst_{1}$
    \item $\myN(\EX \lnot \qst_1) = \EX \qst_{1}$
    \item $\myN(\phi)[\lnot\qst_1] = \phi[\qst_1]$
  \end{itemize}
\end{frame}

\begin{frame}{Find a Solution to $\phi(\qst_1)$}
  \begin{itemize}
    \item find solution for $\myN(\phi[\qst_1])$
    \item negate substitutions \\
      \[
        \llbracket \phi(\qst_1) \rrbracket (s) = \{ \lnot l \mid l \in 
          \llbracket \myN(\phi)[\qst_1] \rrbracket (s) \}
      \]
  \end{itemize}
\end{frame}



\subsection{Mixed Queries}%%%%%%%%%%%%%%%%%%%%%%%%%%%%%%%%%%%%%%%%

\begin{frame}{Decide Mixed Queries}
  Mixed queries $\phi[\qst_1]$:
  \begin{itemize}
    \item transform mixed query into monotone one
    \item apply query checking
    \item postprocess solution
  \end{itemize}
\end{frame}

\begin{frame}{Transform into Monotone Query}
  Transform mixed query $\phi[\qst_1]$ into $\phi[\qst_{1+},\qst_{1-}]$ denoted by $\myH$
  \begin{itemize}
    \item replace positive occurrences with $\qst_{1+}$
    \item replace negative occurrences with $\qst_{1-}$
    \item $\myH(\qst_1 \land \EX \lnot \qst_1) = \qst_{1+} \land \EX \lnot \qst_{1-}$
    \item $\myH$ does not change restrictions \\ 
          $\PF(\qst_{1}) = \PF(\qst_{1+}) = \PF(\qst_{1-})$
  \end{itemize}
\end{frame}

\begin{frame}{Find a Solution to $\phi(\qst_1)$}
  \begin{itemize}
    \item find solution for $\phi[\qst_{1+},\qst_{1-}]$
    \item postprocess solution for $\phi[\qst_{1+},\qst_{1-}]$
      \[
        \llbracket \phi(\qst_1) \rrbracket (s) = \{ a \mid (a,a) \in 
          \llbracket \myH (\phi)[\qst_{1+},\qst_{1-}] \rrbracket (s) \}
      \]
  \end{itemize}
  
  extendable to multiple mixed placeholders
\end{frame}
